theories/terms.v
@@ -9,20 +9,24 @@ From bunched Require Import syntax interp.
 Inductive bterm (var : Type) : Type :=
 | Var (x : var)
 | TComma (T1 T2 : bterm var)
+| TSemic (T1 T2 : bterm var)
 .
 Arguments Var {_} x.
 Arguments TComma {_} T1 T2.
+Arguments TSemic {_} T1 T2.
 
 Global Instance bterm_fmap : FMap bterm :=
   fix go _ _ f T { struct T } := let _ : FMap _ := go in
   match T with
   | Var x => Var (f x)
   | TComma T1 T2 => TComma (f <$> T1) (f <$> T2)
+  | TSemic T1 T2 => TSemic (f <$> T1) (f <$> T2)
   end.
 
 Equations term_fv `{!EqDecision V,!Countable V} (T : bterm V) : gset V :=
   term_fv (Var x) := {[ x ]};
   term_fv (TComma T1 T2) := term_fv T1 ∪ term_fv T2;
+  term_fv (TSemic T1 T2) := term_fv T1 ∪ term_fv T2;
 .
 
 Equations linear_bterm `{!EqDecision V,!Countable V}
@@ -30,13 +34,17 @@ Equations linear_bterm `{!EqDecision V,!Countable V}
   linear_bterm (Var x) := True;
   linear_bterm (TComma T1 T2) :=
     term_fv T1 ## term_fv T2 ∧
-    linear_bterm T1 ∧ linear_bterm T2.
-
+    linear_bterm T1 ∧ linear_bterm T2;
+  linear_bterm (TSemic T1 T2) :=
+    term_fv T1 ## term_fv T2 ∧
+    linear_bterm T1 ∧ linear_bterm T2;
+.
 Fixpoint bterm_ctx_act `{!EqDecision V,!Countable V}
          (T : bterm V) (Δs : V → bunch) : bunch :=
   match T with
   | Var v => Δs v
   | TComma T1 T2 => bterm_ctx_act T1 Δs,, bterm_ctx_act T2 Δs
+  | TSemic T1 T2 => bterm_ctx_act T1 Δs;, bterm_ctx_act T2 Δs
   end%B.
 
 Fixpoint bterm_alg_act {PROP : bi} `{!EqDecision V,!Countable V}
@@ -44,17 +52,15 @@ Fixpoint bterm_alg_act {PROP : bi} `{!EqDecision V,!Countable V}
   match T with
   | Var v => Xs v
   | TComma T1 T2 => bterm_alg_act T1 Xs ∗ bterm_alg_act T2 Xs
+  | TSemic T1 T2 => bterm_alg_act T1 Xs ∧ bterm_alg_act T2 Xs
   end%I.
-
-(** A semimorphism between BI algebras is a function that preserves ∗ and ∧ *)
-Class SemiMorph {A B : bi} (f : A → B) :=
-  { smor_sep (X Y : A) : (f X ∗ f Y)%I ≡ (f (X ∗ Y))%I; }.
 
 Lemma bterm_fmap_compose {A B C} (f : A → B) (g : B → C) (T : bterm A) :
   (g ∘ f) <$> T = g <$> (f <$> T).
 Proof.
   induction T; simpl; auto.
-  rewrite IHT1 IHT2 //.
+  - rewrite IHT1 IHT2 //.
+  - rewrite IHT1 IHT2 //.
 Qed.
 
 Lemma bterm_ctx_act_fv `{!EqDecision V,!Countable V} (T : bterm V) Δs Γs :
@@ -65,14 +71,8 @@ Proof.
   - set_solver.
   - set_unfold. intros H.
     rewrite IHT1; eauto. rewrite IHT2; eauto.
-Qed.
-
-Lemma bterm_morph_commute {A B : bi} `{!EqDecision V, !Countable V}
-      (T : bterm V) (Xs : V → A) (f : A → B) `{!SemiMorph f}:
-  f (bterm_alg_act (PROP:=A) T Xs) ≡ bterm_alg_act (PROP:=B) T (f ∘ Xs).
-Proof.
-  induction T; simpl; first reflexivity.
-  rewrite -IHT1 -IHT2. by rewrite smor_sep.
+  - set_unfold. intros H.
+    rewrite IHT1; eauto. rewrite IHT2; eauto.
 Qed.
 
 Lemma bterm_alg_act_mono {PROP : bi} `{!EqDecision V, !Countable V}
@@ -81,7 +81,7 @@ Lemma bterm_alg_act_mono {PROP : bi} `{!EqDecision V, !Countable V}
   bterm_alg_act T Xs ⊢ bterm_alg_act (PROP:=PROP) T Ys.
 Proof.
   intros HXY. induction T; simpl; auto.
-  by rewrite IHT1 IHT2.
+  all: by rewrite IHT1 IHT2.
 Qed.
 
 Lemma bterm_ctx_alg_act {PROP : bi} `{!EqDecision V,!Countable V}
@@ -91,6 +91,7 @@ Lemma bterm_ctx_alg_act {PROP : bi} `{!EqDecision V,!Countable V}
 Proof.
   induction T; simpl.
   - reflexivity.
+  - by rewrite IHT1 IHT2.
   - by rewrite IHT1 IHT2.
 Qed.
 
@@ -117,6 +118,29 @@ Proof.
       rewrite functions.fn_lookup_insert_ne//.
     + destruct (IHT2 i Hlin2 Hi2) as (Π₁ & HΠ1).
       exists (Π₁++[CtxCommaR (bterm_ctx_act T1 Δs)]).
+      intros Γ. rewrite fill_app /=.
+      rewrite HΠ1. f_equiv.
+      assert (i ∉ term_fv T1).
+      { set_solver. }
+      apply bterm_ctx_act_fv.
+      intros j. destruct (decide (i = j)) as [->|?].
+      { naive_solver. }
+      rewrite functions.fn_lookup_insert_ne//.
+  - destruct Hlin as (Hdisj & Hlin1 & Hlin2).
+    set_unfold.
+    destruct Hi as [Hi1 | Hi2].
+    + destruct (IHT1 i Hlin1 Hi1) as (Π₁ & HΠ1).
+      exists (Π₁++[CtxSemicL (bterm_ctx_act T2 Δs)]).
+      intros Γ. rewrite fill_app /=.
+      rewrite HΠ1. f_equiv.
+      assert (i ∉ term_fv T2).
+      { set_solver. }
+      apply bterm_ctx_act_fv.
+      intros j. destruct (decide (i = j)) as [->|?].
+      { naive_solver. }
+      rewrite functions.fn_lookup_insert_ne//.
+    + destruct (IHT2 i Hlin2 Hi2) as (Π₁ & HΠ1).
+      exists (Π₁++[CtxSemicR (bterm_ctx_act T1 Δs)]).
       intros Γ. rewrite fill_app /=.
       rewrite HΠ1. f_equiv.
       assert (i ∉ term_fv T1).
